Simple Data: go back to exps contexts as a list

proof/Simple_Data/EsContext.v
@@ -6,10 +6,6 @@ Require Export SubstExpExp.
 
 (********************************************************************)
 (** * Evaluation Contexts of lists *)
-(** An evaluation context defines a function that allows us to
-    update a node in the AST for an expression. We use this to
-    update nodes during single step evaluation. *)
-
 (*  A context defined by one place in a list of exps, where all 
     the exps to the left of it in the list are values:
          v0 v1 v2 xx x4 x5 x6
@@ -17,54 +13,37 @@ Require Export SubstExpExp.
     This is useful when enforcing a left-to-right evaluation
     order for a list of exps, like in the arguments of an XCon *)
 Inductive exps_ctx : (exp -> list exp) -> Prop :=
- | XscIx 
-   :  forall ix xs vs x xs'
-   ,  splitAt ix xs = (vs, x :: xs')
-   -> Forall  whnfX vs
-   -> exps_ctx (fun xx => app vs (xx :: xs')).
+ | XscHead
+   :  exps_ctx (fun xx => xx :: nil)
+
+ | XscCons
+   :  forall v C
+   ,  whnfX v
+   -> exps_ctx C
+   -> exps_ctx (fun xx => v :: C xx).
+
+Hint Constructors exps_ctx.
 
 
-Lemma exps_ctx_Forall2 
- :   forall {B: Type} (R: exp -> B -> Prop) 
-            (x: exp)  Cs
-            (y: B)    (ys: list B)
- ,   exps_ctx Cs
- ->  Forall2 R (Cs x) ys
- ->  (exists y, In y ys /\ R x y).
+Lemma context_equiv_exp
+ :  forall C1 C2 x1 x2
+ ,  exps_ctx C1
+ -> exps_ctx C2
+ -> C1 x1 = C2 x2
+ -> x1 = x2.
 Proof.
- intros.
- inverts H.
- assert (In x (vs ++ x :: xs')). apply in_splitted.
- lets D: Forall2_exists_left_In H H0.
- destruct D. 
- exists x1. eauto.
-Qed.  
-
-
-Lemma exps_ctx_Forall2_swap
- :   forall {B: Type} (R: exp -> B -> Prop)
-            (x1 x2 : exp) Cs
-            (y: B)        (ys: list B)
- ,   exps_ctx Cs
- ->  (forall y, R x1 y -> R x2 y)
- ->  Forall2 R (Cs x1) ys
- ->  Forall2 R (Cs x2) ys.
-Proof.
- intros.
- inverts H.
- lets HP: (@splitAt_app_cons exp) H2.
- lets D: Forall2_app_inv_l H1.
-  destruct D as [ys1].
-  destruct H as [ys2].
-  inverts H. inverts H5.
-  apply Forall2_app.
-   auto. clear H1. clear H4.
-  destruct ys2.
-   inverts H.
-   inverts H.
-   apply Forall2_cons.
-    apply H0. auto.
-    auto.
+ intros C1 C2 x1 x2 H1 H2. intros.
+ gen C2.
+  induction H1; intros.
+   inverts H2.
+    inverts H. auto.
+    inverts H1.
+     false. false.
+   inverts H2.
+    inverts H0.
+    inverts H1. false. false.
+   inverts H0.
+   eauto.
 Qed.
 
 
@@ -95,7 +74,7 @@ Inductive exp_ctx : (exp -> exp) -> Prop :=
     we're talking about. *)
  | XcCon 
    :  forall dc C
-   ,  exps_ctx C
+   ,  exps_ctx C 
    -> exp_ctx  (fun xx => XCon dc (C xx))
 
  (* We need to reduce the discriminant of a case to a value. *)
